x86/Asmgenproof.v
@@ -372,10 +372,10 @@ Section WITHINITSPRA.
 
   Variables init_sp init_ra: val.
 
-  Definition match_stackframe_frame_adt s (f: option frame_adt * Z):=
+  Definition match_stackframe_frame_adt s (f: frame_adt):=
     match s, f with
-      Stackframe fn sp _ _, (Some (frame_with_info stk (Some fi)), n) =>
-      stk = sp /\ n = frame_size fi /\
+      Stackframe fn sp _ _, (l, Some fi, n) =>
+      In sp l /\ n = frame_size fi /\
       forall f, Genv.find_funct_ptr ge fn = Some (Internal f) ->
            frame_size fi = Mach.fn_stacksize f /\
            range_eqb (Ptrofs.unsigned (fn_link_ofs f)) (size_chunk Mptr)
@@ -388,13 +388,9 @@ Section WITHINITSPRA.
     | _, _ => False
     end.
 
-  Definition ms_init (f: option frame_adt * Z) :=
+  Definition ms_init (f: frame_adt) :=
     forall b o, init_sp = Vptr b o ->
-           match f with
-             (Some (frame_with_info stk _),n) =>
-             b = stk
-           | _ => False
-           end.
+           frame_blocks f = b :: nil.
 
   Definition ms_nil :=
     forall b o, init_sp = Vptr b o -> False.
@@ -418,7 +414,8 @@ Section WITHINITSPRA.
         (AT: transl_code_at_pc ge (rs PC) fb f c ep tf tc)
         (AG: agree ms (Vptr sp Ptrofs.zero) rs)
         (AXP: ep = true -> rs#RAX = parent_sp init_sp s)
-        (MATCHFRAMES: list_prefix match_stackframe_frame_adt ms_init ms_nil (Stackframe fb sp (Vptr sp Ptrofs.zero) c :: s) (Mem.stack_adt m)),
+        (MATCHFRAMES: list_prefix match_stackframe_frame_adt ms_init ms_nil (Stackframe fb sp (Vptr sp Ptrofs.zero) c :: s) (Mem.stack_adt m))
+        (SAMEADT: list_forall2 (fun f1 f2 => f1 = f2) (Mem.stack_adt m) (Mem.stack_adt m')),
       match_states (Mach.State s fb (Vptr sp Ptrofs.zero) c ms m)
                    (Asm.State rs m')
   | match_states_call:
@@ -428,7 +425,8 @@ Section WITHINITSPRA.
         (AG: agree ms (parent_sp init_sp s) rs)
         (ATPC: rs PC = Vptr fb Ptrofs.zero)
         (ATLR: rs RA = parent_ra init_ra s)
-        (MATCHFRAMES: list_prefix match_stackframe_frame_adt ms_init ms_nil s (Mem.stack_adt m)),
+        (MATCHFRAMES: list_prefix match_stackframe_frame_adt ms_init ms_nil s (Mem.stack_adt m))
+        (SAMEADT: list_forall2 (fun f1 f2 => f1 = f2) (Mem.stack_adt m) (Mem.stack_adt m')),
       match_states (Mach.Callstate s fb ms m)
                    (Asm.State rs m')
   | match_states_return:
@@ -438,7 +436,8 @@ Section WITHINITSPRA.
         (AG: agree ms (parent_sp init_sp s) rs)
         (RA_VUNDEF: rs RA = Vundef)
         (ATPC: rs PC = parent_ra init_ra s)
-        (MATCHFRAMES: list_prefix match_stackframe_frame_adt ms_init ms_nil s (Mem.stack_adt m)),
+        (MATCHFRAMES: list_prefix match_stackframe_frame_adt ms_init ms_nil s (Mem.stack_adt m))
+        (SAMEADT: list_forall2 (fun f1 f2 => f1 = f2) (Mem.stack_adt m) (Mem.stack_adt m')),
       match_states (Mach.Returnstate s ms m)
                    (Asm.State rs m').
 
@@ -453,7 +452,8 @@ Lemma exec_straight_steps:
        exec_straight tge tf c rs1 m1' k rs2 m2'
     /\ agree ms2 (Vptr sp Ptrofs.zero) rs2
     /\ (it1_is_parent ep i = true -> rs2#RAX = parent_sp init_sp s)) ->
-  forall LF2: list_prefix match_stackframe_frame_adt ms_init ms_nil (Stackframe fb sp (Vptr sp Ptrofs.zero) c :: s) (Mem.stack_adt m2),
+  forall (LF2: list_prefix match_stackframe_frame_adt ms_init ms_nil (Stackframe fb sp (Vptr sp Ptrofs.zero) c :: s) (Mem.stack_adt m2))
+                     (SAMEADT: list_forall2 (fun f1 f2 => f1 = f2) (Mem.stack_adt m2) (Mem.stack_adt m2')),
   exists st',
   plus step tge (State rs1 m1') E0 st' /\
   match_states (Mach.State s fb (Vptr sp Ptrofs.zero) c ms2 m2) st'.
@@ -478,7 +478,8 @@ Lemma exec_straight_steps_goto:
        exec_straight tge tf c rs1 m1' (jmp :: k') rs2 m2'
     /\ agree ms2 (Vptr sp Ptrofs.zero) rs2
     /\ exec_instr tge tf jmp rs2 m2' = goto_label tge tf lbl rs2 m2') ->
-  forall LF2:   list_prefix match_stackframe_frame_adt ms_init ms_nil (Stackframe fb sp (Vptr sp Ptrofs.zero) c' :: s) (Mem.stack_adt m2),
+  forall (LF2:   list_prefix match_stackframe_frame_adt ms_init ms_nil (Stackframe fb sp (Vptr sp Ptrofs.zero) c' :: s) (Mem.stack_adt m2))
+    (SAMEADT: list_forall2 (fun f1 f2 => f1 = f2) (Mem.stack_adt m2) (Mem.stack_adt m2')),
   exists st',
   plus step tge (State rs1 m1') E0 st' /\
   match_states (Mach.State s fb (Vptr sp Ptrofs.zero) c' ms2 m2) st'.
@@ -567,7 +568,7 @@ Inductive asm_no_none: state -> Prop :=
 | ann_intro:
     forall rs m
       (NONONE: Forall (fun x => match x with
-                               (None,n) => False
+                               (_,None,n) => False
                              |  _ => True
                              end) (Mem.stack_adt m)),
       asm_no_none (State rs m).
@@ -602,6 +603,7 @@ Inductive asm_no_none: state -> Prop :=
     unfold goto_label in H; repeat destr_in H.
   Qed.
 
+
   Lemma step_asm_no_none:
     forall s1 t s2,
       step tge s1 t s2 ->
@@ -618,9 +620,9 @@ Inductive asm_no_none: state -> Prop :=
               | now (repeat destr_in H8)
               | idtac ].
       + repeat destr_in H8.
+        edestruct Mem.push_frame_alloc_record as (m2 & ALLOC & m3 & STORES & RSB). eauto.
         erewrite Mem.record_stack_blocks_stack_adt. 2: eauto.
-        erewrite Mem.store_stack_blocks. 2: eauto.
-        erewrite Mem.store_stack_blocks. 2: eauto.
+        erewrite Mem.do_stores_stack_adt. 2: eauto.
         erewrite Mem.alloc_stack_blocks; eauto.
       + repeat destr_in H8.
         erewrite <- Mem.free_stack_blocks in NONONE. 2: eauto.
@@ -659,9 +661,10 @@ Inductive asm_no_none: state -> Prop :=
   Lemma check_top_frame_ok:
     forall fb stk ra c s m m' f ,
       list_prefix match_stackframe_frame_adt ms_init ms_nil (Stackframe fb stk ra c :: s) (Mem.stack_adt m) ->
+      list_forall2 (fun f1 f2 => f1 = f2) (Mem.stack_adt m) (Mem.stack_adt m') ->
       Forall (fun x => match x with
-                      (Some _, _) => True
-                    | (None, _) => False
+                      (_,Some _, _) => True
+                    | (_,None, _) => False
                     end) (Mem.stack_adt m') ->
       Mem.extends m m' ->
       Genv.find_funct_ptr ge fb = Some (Internal f) ->
@@ -670,55 +673,61 @@ Inductive asm_no_none: state -> Prop :=
   Proof.
     clear - memory_model_prf init_sp_not_vundef.
     unfold check_top_frame.
-    intros fb stk ra c s m m' f MATCHFRAMES NONONE MEXT FIND PTRZERO.
+    intros fb stk ra c s m m' f MATCHFRAMES SAMEADT NONONE MEXT FIND PTRZERO.
     inv MATCHFRAMES.
     generalize (Mem.extends_stack_adt _ _ MEXT).
-    rewrite <- H. intro A; inv A.
-    rewrite <- H2 in NONONE. inv NONONE.
-    destruct b1; simpl in *. destruct o; try easy.
-    destruct b; simpl in *.
-    destruct o; try easy. destruct f1; try easy. 
-    destruct o; try easy.
+    rewrite <- H. intro A.
+    destr.
+    {
+      inv A. exploit (stack_inject_frames O). constructor; simpl; auto.
+      unfold flat_frameinj. simpl. eauto.
+      intros (f2 & A & B). inv A. simpl in H0. congruence.
+    }
+    inv NONONE. destruct f0, p.
+    destruct o; destruct H2. 
+    
     Ltac clean:=
       repeat match goal with
                H : _ /\ _ |- _ => destruct H; subst
              | H: True |- _ => clear H
              end.
+    red in PAB. destruct b, p. destruct o. 2: inv PAB.
     clean.
-    inv H0.
-    generalize (INJ _ _ eq_refl). intros; subst.
-    specialize (H3 _ FIND).
-    destruct H3 as (SEQ & LEQ & REQ & OTHER).
+    exploit (stack_inject_frames _ _ _ _ _ A O); eauto.
+    constructor; simpl; auto.
+    unfold flat_frameinj; simpl. auto.
+    intros (f2 & FAP & FI). inv FAP. simpl in H1. inv H1.
+    destruct FI.
+    rewrite Forall_forall in frame_inject_inj.
+    specialize (frame_inject_inj _ H0 _ _ eq_refl). simpl in frame_inject_inj.
+    red in frame_inject_frame. simpl in frame_inject_frame.
+    rewrite Forall_forall in frame_inject_frame.
+    specialize (frame_inject_frame _ H0 _ _ eq_refl).
+    specialize (H2 _ FIND).
+    destruct H2 as (SEQ & LEQ & REQ & OTHER).
+    rewrite <- H in SAMEADT. inv SAMEADT. simpl in H5. inv H5.
     rewrite SEQ, LEQ , REQ.
     rewrite <- ! andb_assoc. rewrite OTHER.
-    rewrite if_peq, ? if_zeq, ? if_zeq'. simpl.
-    inv H4; inv H6. inv LPrec. simpl. destruct (init_sp) eqn:?; auto.
-    edestruct PNIL; eauto.
-    destruct b1; simpl in *.
-    destruct o; try easy.
-    destruct a1; simpl in *.
-    destruct o; try easy.
-    clean.
-    inv LPrec. simpl; auto. destruct init_sp eqn:?; auto.
-    red in PINIT. rewrite Heqv in PINIT. 
-    specialize (PINIT _ _ eq_refl).
-    destruct f2; try easy. inv H0.
-    specialize (PTRZERO _ _ eq_refl). subst.
-    destruct (peq b0 b2). simpl. destruct (Ptrofs.eq_dec Ptrofs.zero Ptrofs.zero); try discriminate. simpl. auto. congruence.
-    exfalso; apply n. eapply FB0. reflexivity.
-    specialize (PTRZERO _ _ eq_refl). subst.
-    destruct (peq b0 b2). simpl. destruct (Ptrofs.eq_dec Ptrofs.zero Ptrofs.zero); try discriminate. simpl. auto. congruence.
-    exfalso; apply n. eapply INJ0. reflexivity. auto.
-    simpl.
-    red in PAB.
-    destruct a.
-    destruct f2; try easy.
-    destruct o; try easy.
-    destruct PAB as (? & ? & PAB). subst.
-    inv H0. simpl.
-    erewrite <- INJ0. 2: reflexivity.
-    rewrite if_peq.
-    destruct (Ptrofs.eq_dec Ptrofs.zero Ptrofs.zero); try discriminate. simpl. auto. congruence.
+    destruct (in_dec peq stk l0). 2: exfalso; apply n; auto. 
+    simpl. rewrite ! if_zeq.
+    inv LPrec.
+    + simpl. destruct (init_sp) eqn:?; auto.
+      edestruct PNIL; eauto.
+    + simpl. red in PINIT.
+      destruct init_sp eqn:?; auto.
+      specialize (PINIT _ _ eq_refl). inv H7.
+      rewrite PINIT. destr.  apply andb_false_iff in Heqb0.
+      destruct Heqb0. simpl in H1. destr_in H1. discriminate. 
+      specialize (PTRZERO _ _ eq_refl). subst. discriminate.
+    + simpl. 
+      red in PAB.
+      destruct a, b, p.
+      destruct o; try easy.
+      destruct PAB as (? & ? & PAB). subst.
+      inv H7. simpl. destr.
+      apply andb_false_iff in Heqb.
+      destruct Heqb. destruct (in_dec peq sp l2). discriminate. exfalso; apply n. auto. 
+      discriminate.
   Qed.
 
   
@@ -764,7 +773,11 @@ Local Transparent destroyed_by_setstack.
   eapply msfa_ext_code; eauto.
   unfold Mem.storev in H; destr_in H. 
   erewrite Mem.store_no_abstract; eauto.
-  
+  unfold Mem.storev in H; destr_in H.
+  simpl in A. 
+  apply Mem.store_no_abstract in H; eauto.
+  apply Mem.store_no_abstract in A; eauto.
+  congruence.
 - (* Mgetparam *)
   assert (f0 = f) by congruence; subst f0.
   unfold load_stack in *.
@@ -839,6 +852,11 @@ Opaque loadind.
   eapply msfa_ext_code; eauto.
   unfold Mem.storev in H0; destr_in H0.
   erewrite Mem.store_no_abstract; eauto.
+  unfold Mem.storev in H0; destr_in H0.
+  unfold Mem.storev in C; destr_in C.
+  apply Mem.store_no_abstract in H0; eauto.
+  apply Mem.store_no_abstract in C; eauto.
+  congruence.
 
 - (* Mcall *)
   assert (f0 = f) by congruence.  subst f0.
@@ -941,6 +959,12 @@ Opaque loadind.
   edestruct Mem.unrecord_stack_adt as (b0 & EQ'). apply H4.
   erewrite Mem.free_stack_blocks in EQ'. 2: eauto.
   rewrite EQ' in MATCHFRAMES; inv MATCHFRAMES; auto.
+  edestruct Mem.unrecord_stack_adt as (b0 & EQ'). apply H4.
+  erewrite Mem.free_stack_blocks in EQ'. 2: eauto.
+  edestruct Mem.unrecord_stack_adt as (b1 & EQ''). apply G.
+  erewrite Mem.free_stack_blocks in EQ''. 2: eauto.
+  rewrite EQ', EQ'' in SAMEADT. inv SAMEADT; auto.
+
 
 + (* Direct call *)
   generalize (code_tail_next_int _ _ _ _ NOOV H9). intro CT1.
@@ -966,7 +990,12 @@ Opaque loadind.
   edestruct Mem.unrecord_stack_adt as (b0 & EQ'). apply H4.
   erewrite Mem.free_stack_blocks in EQ'. 2: eauto.
   rewrite EQ' in MATCHFRAMES; inv MATCHFRAMES; auto.
-  
+  edestruct Mem.unrecord_stack_adt as (b0 & EQ'). apply H4.
+  erewrite Mem.free_stack_blocks in EQ'. 2: eauto.
+  edestruct Mem.unrecord_stack_adt as (b1 & EQ''). apply G.
+  erewrite Mem.free_stack_blocks in EQ''. 2: eauto.
+  rewrite EQ', EQ'' in SAMEADT. inv SAMEADT; auto.
+
 - (* Mbuiltin *)
   inv AT. monadInv H4.
   exploit functions_transl; eauto. intro FN.
@@ -997,6 +1026,10 @@ Opaque loadind.
   congruence.
   eapply msfa_ext_code; eauto.
   erewrite <- external_call_stack_blocks; eauto.
+  replace (Mem.stack_adt m') with (Mem.stack_adt m).
+  replace (Mem.stack_adt m2') with (Mem.stack_adt m'0). auto.
+  eapply external_call_stack_blocks; eauto.
+  eapply external_call_stack_blocks; eauto.
 - (* Mgoto *)
   assert (f0 = f) by congruence. subst f0.
   inv AT. monadInv H4.
@@ -1144,7 +1177,11 @@ Transparent destroyed_by_jumptable.
   edestruct Mem.unrecord_stack_adt as (b0 & EQ'). apply H3.
   erewrite Mem.free_stack_blocks in EQ'. 2: eauto.
   rewrite EQ' in MATCHFRAMES; inv MATCHFRAMES; auto.
-  
+  edestruct Mem.unrecord_stack_adt as (b0 & EQ'). apply H3.
+  erewrite Mem.free_stack_blocks in EQ'. 2: eauto.
+  edestruct Mem.unrecord_stack_adt as (b1 & EQ''). apply G.
+  erewrite Mem.free_stack_blocks in EQ''. 2: eauto.
+  rewrite EQ', EQ'' in SAMEADT. inv SAMEADT; auto.  
 - (* internal function *)
   exploit functions_translated; eauto. intros [tf [A B]]. monadInv B.
   generalize EQ; intros EQ'. monadInv EQ'.
@@ -1157,6 +1194,7 @@ Transparent destroyed_by_jumptable.
   intros [m2' [F G]].
   exploit Mem.storev_extends. eexact G. eexact H3. eauto. eauto.
   intros [m3' [P Q]].
+  exploit frame_size_correct. eauto. intros (X & Y). 
   exploit Mem.record_stack_blocks_extends.
   apply Q. eauto.
   {
@@ -1164,28 +1202,44 @@ Transparent destroyed_by_jumptable.
     erewrite Mem.store_stack_blocks. 2: simpl in *; eauto.
     erewrite Mem.store_stack_blocks. 2: simpl in *; eauto.
     erewrite Mem.alloc_stack_blocks; eauto. intro INF. apply Mem.in_frames_valid in INF.
-    eapply Mem.fresh_block_alloc in INF; eauto.
+    red in H5; simpl in H5.
+    intuition subst.
+    eapply Mem.fresh_block_alloc in INF; eauto. 
+  }
+  {
+    constructor; auto.
+    simpl; intros. inv H6.
+    eapply Mem.perm_store_2 in H5. 2: simpl in *; eauto.
+    eapply Mem.perm_store_2 in H5. 2: simpl in *; eauto.
+    eapply Mem.perm_alloc_inv in H5. 2: eauto. rewrite pred_dec_true in H5; auto.
+    rewrite X. auto. 
   }
   intros (m1'' & CC & DD).
+  exploit Mem.alloc_record_push_frame. rewrite X. eauto.
+  instantiate (2:= (chunk_of_type Tptr, fn_link_ofs f, (parent_sp init_sp s))::(chunk_of_type Tptr, fn_retaddr_ofs f, parent_ra init_ra s)::nil).
+  simpl. simpl in F. rewrite Ptrofs.add_zero_l in F. rewrite F.
+  simpl in P. rewrite Ptrofs.add_zero_l in P. rewrite P. eauto. rewrite X. eauto.
+  intro PF.
   left; econstructor; split.
   apply plus_one. econstructor; eauto.
   simpl. rewrite Ptrofs.unsigned_zero. simpl. eauto.
   simpl.
-  generalize (frame_size_correct _ _ H). intros (SEQ & LEQ).
-  rewrite SEQ.
-  rewrite C. simpl in F, P.
-  replace (chunk_of_type Tptr) with Mptr in F, P by (unfold Tptr, Mptr; destruct Archi.ptr64; auto).
-  rewrite (sp_val _ _ _ AG) in F. rewrite F.
-  rewrite ATLR. rewrite P.
-  unfold check_alloc_frame. rewrite LEQ.
+  change Mptr with (chunk_of_type Tptr).
+  rewrite ATLR. erewrite agree_sp. 2: eauto. rewrite PF.
+  (* rewrite X. *)
+  (* generalize (frame_size_correct _ _ H). intros (SEQ & LEQ). *)
+  (* rewrite SEQ. *)
+  (* rewrite C. simpl in F, P. *)
+  (* replace (chunk_of_type Tptr) with Mptr in F, P by (unfold Tptr, Mptr; destruct Archi.ptr64; auto). *)
+  (* rewrite (sp_val _ _ _ AG) in F. rewrite F. *)
+  (* rewrite ATLR. rewrite P. *)
+  unfold check_alloc_frame. rewrite Y. 
   move H0 at bottom.
   unfold Mach.check_alloc_frame in H0.
   destruct H0 as (LRRO & LRDISJ & EQlink).
   rewrite if_zeq.
-  rewrite LEQ in LRDISJ.
-  rewrite LRDISJ. 
-  rewrite CC.
-  eauto.
+  rewrite Y in LRDISJ.
+  rewrite LRDISJ. eauto.
   econstructor; eauto.
   unfold nextinstr. rewrite Pregmap.gss. repeat rewrite Pregmap.gso; auto with asmgen.
   rewrite ATPC. simpl. constructor; eauto.
@@ -1197,18 +1251,16 @@ Transparent destroyed_at_function_entry.
   simpl; intros. apply Pregmap.gso; auto with asmgen. tauto.
   congruence.
   constructor.
-  intros. Simplifs. eapply agree_sp; eauto.
-  unfold Mem.storev in H4, H3. destr_in H4. destr_in H3.
   erewrite Mem.record_stack_blocks_stack_adt. 2: eauto.
   constructor; auto.
-  erewrite Mem.store_stack_blocks. 2: eauto.
+  erewrite Mem.store_stack_blocks. 2: simpl in * ; eauto.
   erewrite Mem.store_stack_blocks. 2: simpl in *; eauto.
   erewrite Mem.alloc_stack_blocks. 2: eauto.
   auto.
-  generalize (frame_size_correct _ _ H). intros (SEQ & LEQ).
-  constructor; auto.
+  constructor; auto. simpl; auto.
+  rewrite X, H. 
   split; auto.
-  rewrite H. inversion 1. subst.
+  inversion 1. subst. 
   unfold Mach.check_alloc_frame in H0.
   move H0 at bottom.
   split; auto. rewrite <- and_assoc. split.
@@ -1216,12 +1268,22 @@ Transparent destroyed_at_function_entry.
   generalize (size_chunk_pos Mptr); omega.
   generalize (size_chunk_pos Mptr); omega.
   intros.
-  apply H0 in H5.
+  apply H0 in H6.
   destruct (frame_readonly_dec (Mach.fn_frame f0) o); auto.
   apply andb_true_iff. split.
-  rewrite LEQ. destruct zeq; auto.
-  destruct H0. destruct H5. auto.
+  rewrite Y. destruct zeq; auto.
+  destruct H0. destruct H6. auto.
 
+  erewrite (Mem.record_stack_blocks_stack_adt _ _ m1_). 2: eauto.
+  erewrite (Mem.record_stack_blocks_stack_adt _ _ m1''). 2: eauto.
+  constructor; auto.
+  erewrite (Mem.store_stack_blocks _ _ _ _ _ m3). 2: simpl in * ; eauto.
+  erewrite (Mem.store_stack_blocks _ _ _ _ _ m3'). 2: simpl in * ; eauto.
+  erewrite (Mem.store_stack_blocks _ _ _ _ _ m2). 2: simpl in * ; eauto.
+  erewrite (Mem.store_stack_blocks _ _ _ _ _ m2'). 2: simpl in * ; eauto.
+  erewrite (Mem.alloc_stack_blocks _ _ _ m1). 2: eauto.
+  erewrite (Mem.alloc_stack_blocks _ _ _ m1'). 2: eauto.  
+  auto.
 
 - (* external function *)
   exploit functions_translated; eauto.
@@ -1262,6 +1324,11 @@ Transparent destroyed_at_function_entry.
   apply agree_undef_regs_parallel; auto.
   simpl; intros; intuition subst; reflexivity.
   erewrite <- external_call_stack_blocks; eauto.
+  replace (Mem.stack_adt m') with (Mem.stack_adt m). 
+  replace (Mem.stack_adt m2') with (Mem.stack_adt m'0). auto.
+  eapply external_call_stack_blocks; eauto.
+  eapply external_call_stack_blocks; eauto.
+
 - (* return *)
   inv STACKS. simpl in *.
   right. split. omega. split. auto.
@@ -1295,6 +1362,7 @@ Proof.
   destruct (Mem.stack_adt m0). constructor.
   red; intros. inv H3.
   constructor. red; simpl; intros. inv H3.
+  erewrite Genv.init_mem_stack_adt; eauto.  constructor.
   econstructor. erewrite Genv.init_mem_stack_adt; eauto. 
   unfold Genv.symbol_address.
   rewrite (match_program_main TRANSF).
